PhysLean/StringTheory/FTheory/SU5U1/Potential/Irreducible/Basic.lean
@@ -12,26 +12,26 @@ namespace SU5U1
 namespace Charges
 
 def IsIrreducible (x : Charges) (T : PotentialTerm) : Prop :=
-  ∀ y ∈ x.powerset, y = x ↔ y.IsPresent T
+  ∀ y ∈ x.powerset, y = x ↔ y.AllowsTerm T
 
 instance (x : Charges) (T : PotentialTerm) : Decidable (x.IsIrreducible T) :=
-  inferInstanceAs (Decidable (∀ y ∈ powerset x, y = x ↔ y.IsPresent T))
+  inferInstanceAs (Decidable (∀ y ∈ powerset x, y = x ↔ y.AllowsTerm T))
 
 variable {T : PotentialTerm} {x : Charges}
 
-lemma isPresent_of_isIrreducible (h : x.IsIrreducible T) : x.IsPresent T := by
+lemma allowsTerm_of_isIrreducible (h : x.IsIrreducible T) : x.AllowsTerm T := by
   simp only [IsIrreducible] at h
   simpa using h x (self_mem_powerset x)
 
-lemma isPresent_of_has_isIrreducible_subset (hx : ∃ y ∈ powerset x, y.IsIrreducible T) :
-    x.IsPresent T := by
+lemma allowsTerm_of_has_isIrreducible_subset (hx : ∃ y ∈ powerset x, y.IsIrreducible T) :
+    x.AllowsTerm T := by
   obtain ⟨y, hy⟩ := hx
   simp only [mem_powerset_iff_subset] at hy
-  apply isPresent_of_subset hy.1
-  exact isPresent_of_isIrreducible hy.2
+  apply allowsTerm_of_subset hy.1
+  exact allowsTerm_of_isIrreducible hy.2
 
 lemma isIrreducible_iff_powerset_filter_eq :
-    x.IsIrreducible T ↔ x.powerset.filter (fun y => y.IsPresent T) = {x} := by
+    x.IsIrreducible T ↔ x.powerset.filter (fun y => y.AllowsTerm T) = {x} := by
   constructor
   · intro h
     ext y
@@ -58,38 +58,38 @@ lemma isIrreducible_iff_powerset_filter_eq :
       · exact h1
 
 lemma isIrreducible_iff_powerset_countP_eq_one  :
-    x.IsIrreducible T ↔ x.powerset.val.countP (fun y => y.IsPresent T) = 1 := by
+    x.IsIrreducible T ↔ x.powerset.val.countP (fun y => y.AllowsTerm T) = 1 := by
   rw [isIrreducible_iff_powerset_filter_eq]
   constructor
   · intro h
-    trans (Finset.filter (fun y => y.IsPresent T) x.powerset).card
-    · change _ = (Multiset.filter (fun y => y.IsPresent T) x.powerset.val).card
-      exact Multiset.countP_eq_card_filter (fun y => y.IsPresent T) x.powerset.val
+    trans (Finset.filter (fun y => y.AllowsTerm T) x.powerset).card
+    · change _ = (Multiset.filter (fun y => y.AllowsTerm T) x.powerset.val).card
+      exact Multiset.countP_eq_card_filter (fun y => y.AllowsTerm T) x.powerset.val
     · rw [h]
       simp
   · intro h
-    have h1 : (Multiset.filter (fun y => y.IsPresent T) x.powerset.val).card = 1 := by
+    have h1 : (Multiset.filter (fun y => y.AllowsTerm T) x.powerset.val).card = 1 := by
       rw [← h]
-      exact Eq.symm (Multiset.countP_eq_card_filter (fun y => y.IsPresent T) x.powerset.val)
+      exact Eq.symm (Multiset.countP_eq_card_filter (fun y => y.AllowsTerm T) x.powerset.val)
     rw [Multiset.card_eq_one] at h1
     obtain ⟨a, ha⟩ := h1
-    have haMem : a ∈ Multiset.filter (fun y => y.IsPresent T) x.powerset.val := by
+    have haMem : a ∈ Multiset.filter (fun y => y.AllowsTerm T) x.powerset.val := by
       simp [ha]
     simp at haMem
-    have hxMem : x ∈ Multiset.filter (fun y => y.IsPresent T) x.powerset.val := by
-      simpa using isPresent_of_subset haMem.1 haMem.2
+    have hxMem : x ∈ Multiset.filter (fun y => y.AllowsTerm T) x.powerset.val := by
+      simpa using allowsTerm_of_subset haMem.1 haMem.2
     rw [ha] at hxMem
     simp at hxMem
     subst hxMem
     exact Finset.val_inj.mp ha
 
-lemma subset_isIrreducible_of_isPresent
-    (hx : x.IsPresent T) : ∃ y ∈ powerset x, y.IsIrreducible T := by
-  have hPresent : (x.powerset.filter (fun y => y.IsPresent T)) ≠ ∅ := by
+lemma subset_isIrreducible_of_allowsTerm
+    (hx : x.AllowsTerm T) : ∃ y ∈ powerset x, y.IsIrreducible T := by
+  have hPresent : (x.powerset.filter (fun y => y.AllowsTerm T)) ≠ ∅ := by
     rw [← @Finset.nonempty_iff_ne_empty]
     use x
     simp [hx]
-  obtain ⟨y, h1, h2⟩ := min_exists (x.powerset.filter (fun y => y.IsPresent T)) hPresent
+  obtain ⟨y, h1, h2⟩ := min_exists (x.powerset.filter (fun y => y.AllowsTerm T)) hPresent
   use y
   simp at h1
   simp_all
@@ -101,15 +101,15 @@ lemma subset_isIrreducible_of_isPresent
   intro hzy hzpres
   exact subset_trans hzy h1.1
 
-lemma isPresent_iff_subset_isIrreducible :
-    x.IsPresent T ↔ ∃ y ∈ powerset x, y.IsIrreducible T :=
-  ⟨fun h => subset_isIrreducible_of_isPresent h, fun h => isPresent_of_has_isIrreducible_subset h⟩
+lemma allowsTerm_iff_subset_isIrreducible :
+    x.AllowsTerm T ↔ ∃ y ∈ powerset x, y.IsIrreducible T :=
+  ⟨fun h => subset_isIrreducible_of_allowsTerm h, fun h => allowsTerm_of_has_isIrreducible_subset h⟩
 
 lemma card_le_degree_of_isIrreducible (h : x.IsIrreducible T) :
     x.card ≤ T.degree := by
   obtain ⟨y, y_mem_power, y_card,y_present⟩ :=
-    subset_card_le_degree_isPresent_of_isPresent (isPresent_of_isIrreducible h)
-  have hy : y ∈ x.powerset.filter (fun y => y.IsPresent T)  := by
+    subset_card_le_degree_allowsTerm_of_allowsTerm (allowsTerm_of_isIrreducible h)
+  have hy : y ∈ x.powerset.filter (fun y => y.AllowsTerm T)  := by
     simp_all
   rw [isIrreducible_iff_powerset_filter_eq] at h
   rw [h] at hy
@@ -117,12 +117,12 @@ lemma card_le_degree_of_isIrreducible (h : x.IsIrreducible T) :
   subst hy
   exact y_card
 
-lemma eq_isPresentForm_of_isIrreducible (h1 : x.IsIrreducible T) :
-    ∃ a b c, x = isPresentForm a b c T := by
-  obtain ⟨a, b, c,  h2, h3⟩ := isPresentForm_subset_isPresent_of_isPresent
-    (isPresent_of_isIrreducible h1)
+lemma eq_allowsTermForm_of_isIrreducible (h1 : x.IsIrreducible T) :
+    ∃ a b c, x = allowsTermForm a b c T := by
+  obtain ⟨a, b, c,  h2, h3⟩ := allowsTermForm_subset_allowsTerm_of_allowsTerm
+    (allowsTerm_of_isIrreducible h1)
   use a, b, c
-  have hy : isPresentForm a b c T ∈ x.powerset.filter (fun y => y.IsPresent T)  := by
+  have hy : allowsTermForm a b c T ∈ x.powerset.filter (fun y => y.AllowsTerm T)  := by
     simp_all
   rw [isIrreducible_iff_powerset_filter_eq] at h1
   rw [h1] at hy
@@ -130,19 +130,19 @@ lemma eq_isPresentForm_of_isIrreducible (h1 : x.IsIrreducible T) :
   exact hy.symm
 
 open PotentialTerm in
-lemma isPresentForm_isIrreducible  {a b c  : ℤ} {T : PotentialTerm}
+lemma allowsTermForm_isIrreducible  {a b c  : ℤ} {T : PotentialTerm}
     (hT : T ≠ W1 ∧ T ≠ W2) :
-    IsIrreducible (isPresentForm a b c T) T := by
+    IsIrreducible (allowsTermForm a b c T) T := by
   simp [IsIrreducible]
   intro y hy
   constructor
   · intro h
     subst h
-    exact isPresentForm_isPresent
+    exact allowsTermForm_allowsTerm
   · intro h
-    obtain ⟨a', b', c', hsub, hIsPresent⟩ := isPresentForm_subset_isPresent_of_isPresent h
-    have hEq : isPresentForm a' b' c' T  = isPresentForm a b c T :=
-      isPresentForm_eq_of_subset (subset_trans hsub hy) hT
+    obtain ⟨a', b', c', hsub, hAllowsTerm⟩ := allowsTermForm_subset_allowsTerm_of_allowsTerm h
+    have hEq : allowsTermForm a' b' c' T  = allowsTermForm a b c T :=
+      allowsTermForm_eq_of_subset (subset_trans hsub hy) hT
     apply subset_antisymm hy
     rw [← hEq]
     exact hsub
